WIP examples

ml_sources/examples/transactional_consistency/read_committed/examples/dirty_read/dirty_read_code.ml
@@ -1,0 +1,44 @@
+open !Ast
+open Serialization_code
+open Snapshot_isolation_code
+open Util_code
+
+let transaction1 cst =
+  start cst;
+  write cst "x" 1;
+  let vy = read cst "y" in
+  if (vy = Some 1) then (
+    write cst "a" 1;
+  );
+  commitU cst
+
+let transaction2 cst =
+  start cst;
+  write cst "y" 1;
+  let vx = read cst "x" in
+  if (vx = Some 1) then (
+    write cst "b" 1;
+  );
+  commitU cst
+
+let transaction3 cst =
+  start cst;
+  let va = read cst "a" in
+  let vb = read cst "b" in
+  assert (not (va = Some 1 && vb = Some 1));
+  commitU cst
+
+let transaction1_client caddr kvs_addr =
+  let cst = init_client_proxy int_serializer caddr kvs_addr in
+  transaction1 cst
+
+let transaction2_client caddr kvs_addr =
+  let cst = init_client_proxy int_serializer caddr kvs_addr in
+  transaction2 cst
+
+let transaction3_client caddr kvs_addr =
+  let cst = init_client_proxy int_serializer caddr kvs_addr in
+  transaction3 cst
+
+let server srv =
+  init_server int_serializer srv
