ml_sources/examples/transactional_consistency/snapshot_isolation/examples/bank_transfer/bank_transfer_code.ml
@@ -3,12 +3,12 @@ open Serialization_code
 open Snapshot_isolation_code
 open Util_code
 
-let transaction1 cst amount src dst =
+let transaction cst amount src dst =
   start cst;
-  let vsrc = read cst src in
+  let vsrc = unSOME (read cst src) in
   if (amount <= vsrc) then (
     write cst src (vsrc - amount);
-    let vdst = read cst dst in
+    let vdst = unSOME (read cst dst) in
     write cst dst (vdst + amount)
-  )
+  );
   commitU cst
