aneris/examples/transactional_consistency/snapshot_isolation/examples/bank_transfer/bank_transfer_proof.v
@@ -1,0 +1,121 @@
+(* From aneris.aneris_lang Require Import network resources proofmode.
+From aneris.aneris_lang.lib Require Import
+     list_proof inject lock_proof.
+From aneris.aneris_lang.lib.serialization
+     Require Import serialization_proof.
+From aneris.aneris_lang.program_logic Require Import lightweight_atomic.
+From aneris.aneris_lang Require Import tactics proofmode adequacy.
+From trillium.prelude Require Import finitary.
+From aneris.aneris_lang.program_logic Require Import
+     aneris_weakestpre aneris_adequacy aneris_lifting.
+From iris.base_logic.lib Require Import invariants.
+From aneris.examples.transactional_consistency.snapshot_isolation.specs Require Import
+  time events aux_defs resources specs.
+From aneris.examples.transactional_consistency.snapshot_isolation.examples.bank_transfer
+  Require Import bank_transfer_code.
+Import ser_inj.
+From aneris.examples.transactional_consistency.snapshot_isolation.instantiation Require Import
+     snapshot_isolation_api_implementation
+     instantiation_of_init.
+From aneris.examples.transactional_consistency.snapshot_isolation.util Require Import util_proof.
+From iris.algebra Require Import excl.
+From aneris.examples.transactional_consistency.snapshot_isolation.examples Require Import proof_resources.
+From aneris.examples.transactional_consistency Require Import resource_algebras user_params.
+
+Section proof.
+
+  Context `{!User_params, !anerisG Mdl Σ, !SI_resources Mdl Σ, !KVSG Σ}.
+
+  Definition client_inv src dst : iProp Σ :=
+    ∃ (h_src h_dst : Hist) (v_src v_dst : nat), src ↦ₖ (h_src ++ [$v_src]) ∗ dst ↦ₖ (h_dst ++ [$v_dst]).
+
+  Lemma transfer_transaction (amount : nat) (c : val) (src dst : Key) 
+    (client_addr : socket_address) (client_inv_name : namespace) :
+    SI_client_toolbox -∗
+    {{{ ⌜src ∈ KVS_keys⌝ ∗ ⌜dst ∈ KVS_keys⌝ ∗ ⌜src ≠ dst⌝ ∗ 
+        (* ⌜KVS_InvName ⊆ ⊤ ∖ client_inv_name⌝ ∗ *)
+        inv client_inv_name (client_inv src dst) ∗ 
+        ConnectionState c client_addr CanStart  ∗ 
+        IsConnected c client_addr }}}
+      transaction c $amount $src $dst @[ip_of_address client_addr]
+    {{{ v, RET v; True }}}.
+  Proof.
+    iIntros "(#Hinit_kvs & #Hinit_cli & #Hrd & #Hwr & #Hst & #Hcom) %Φ !> 
+    (%Hin & %Hin' & %Hneq & #Hinv & Hstate & #Hconn) HΦ".
+    rewrite /transaction. wp_pures. 
+    wp_apply ("Hst" $! c client_addr (⊤ ∖ ↑client_inv_name)); try solve_ndisj.
+    (* Search (_ ⊆ _). *)
+    (* iPureIntro. set_solver. *)
+    admit.
+    iInv (client_inv_name) as ">[%h_src [%h_dst [%v_src [%v_dst (Hks & Hkd)]]]]" "Hclose".
+    iModIntro. iFrame.
+    iExists {[src := (h_src ++ [$ v_src]); dst := (h_dst ++ [$ v_dst])]}.
+    rewrite !big_sepM_insert; try set_solver. 
+    2 : by apply lookup_singleton_ne.
+    2 : by apply lookup_singleton_ne.
+    2 : by apply lookup_singleton_ne.
+    rewrite big_sepM_empty.
+    iSplitL "Hks Hkd"; first iFrame.
+    iNext. iIntros "(Hcstate & (Hks & Hkd & _) & ((Hcs1 & Hcs2) & (Hcd1 & Hcd2) & _) & _)".
+    iMod ("Hclose" with "[Hks Hkd]") as "_".
+    { iNext. iExists _,_ ,_ , _. iFrame. }
+    iModIntro. wp_pures.
+    wp_apply ("Hrd" $! _ _ ⊤ with "[//][][$]"); first by iPureIntro.
+    iModIntro.
+    iExists _.
+    iFrame.
+    iNext.
+    iIntros "Hcs1".
+    iModIntro.
+    do 2 rewrite last_snoc.
+    rewrite /unSOME.
+    wp_pures.
+    (* wp_op. *)
+    (* case_bool_decide. *)
+    (* destruct (bin_op_eval LeOp amount v_src) eqn:asd. *)
+    case_bool_decide as Hleq.
+    - wp_pures.
+      admit.
+    - wp_pures.
+    Search "case_bool_decide".
+    wp_op.
+    {
+      unfold bin_op_eval.
+    }
+    Search "bin_op_eval_".
+    (* wp_op; try done. *)
+    wp_apply ("Hwr" $! _ _  ⊤ _ (SerVal #1) with "[//][][$]"); first set_solver.
+    iModIntro.
+    iExists _, _.
+    iFrame.
+    iNext.
+    iIntros "(Hcx1 & Hcx2)".
+    iModIntro.
+    wp_pures.
+    wp_apply (commitT_spec rpc client_1_addr (⊤ ∖ ↑client_inv_name));
+    try solve_ndisj. iFrame "#".
+    iInv (client_inv_name) as ">[%h' (Hkx & [-> | (_ & Htok') ])]" "Hclose";
+    try iDestruct (token_exclusive with "Htok Htok'") as "[]".
+    iModIntro.
+    iExists {["x" := []]} , _, {["x" := (Some #1, true)]}.
+    iFrame.
+    iSplitL "Hcx1 Hcx2 Hkx".
+      + iSplitR. iPureIntro. set_solver.
+        iSplitR. iPureIntro. set_solver.
+        iSplitL "Hkx".
+        rewrite !big_sepM_insert; try set_solver.
+        rewrite !big_sepM_insert; try set_solver.
+        rewrite !big_sepM_empty. iFrame.
+      + iNext. iIntros "[_ HBig]".
+        iMod ("Hclose" with "[HBig Htok]") as "_".
+            * iNext. iExists _.
+              rewrite !(big_sepM2_insert); try set_solver.
+              iDestruct "HBig" as "((Hkx & _) & _)".
+              iFrame.
+              iRight.
+              iFrame.
+              by iPureIntro.
+            * iModIntro. by iApply "HΦ".
+  Qed.
+
+End proof. *)
