aneris/examples/transactional_consistency/snapshot_isolation/examples/write_skew/write_skew_proof.v
@@ -1,0 +1,338 @@
+From aneris.aneris_lang Require Import network resources proofmode.
+From aneris.aneris_lang.lib Require Import
+     list_proof inject lock_proof.
+From aneris.aneris_lang.lib.serialization
+     Require Import serialization_proof.
+From aneris.aneris_lang.program_logic Require Import lightweight_atomic.
+From aneris.aneris_lang Require Import tactics proofmode adequacy.
+From trillium.prelude Require Import finitary.
+From aneris.aneris_lang.program_logic Require Import
+     aneris_weakestpre aneris_adequacy aneris_lifting.
+From iris.base_logic.lib Require Import invariants.
+From aneris.examples.transactional_consistency.snapshot_isolation.specs Require Import
+  time events aux_defs resources specs.
+From aneris.examples.transactional_consistency.snapshot_isolation.examples.write_skew
+  Require Import write_skew_code.
+Import ser_inj.
+From aneris.examples.transactional_consistency.snapshot_isolation.instantiation Require Import
+     snapshot_isolation_api_implementation
+     instantiation_of_init.
+From aneris.examples.transactional_consistency.snapshot_isolation.util Require Import util_proof.
+From iris.algebra Require Import excl.
+From aneris.examples.transactional_consistency.snapshot_isolation.examples Require Import proof_resources.
+From aneris.examples.transactional_consistency Require Import resource_algebras user_params.
+
+Definition server_addr := SocketAddressInet "0.0.0.0" 80.
+Definition client_1_addr := SocketAddressInet "0.0.0.1" 80.
+Definition client_2_addr := SocketAddressInet "0.0.0.2" 80.
+
+Instance params : User_params :=
+{| KVS_address := server_addr;
+  KVS_keys := {["x"; "y"]};
+  KVS_InvName := nroot .@ "siinv";
+  KVS_serialization := int_serialization;
+  KVS_ser_inj := int_ser_is_ser_injective;
+  KVS_ser_inj_alt := int_ser_is_ser_injective_alt
+|}.
+
+Definition client_inv_name := nroot.@"clinv".
+
+Section proofs.
+
+Context `{!anerisG Mdl Σ, !SI_resources Mdl Σ, !KVSG Σ}.
+
+  Definition client_inv (γF1 γF2 : gname): iProp Σ :=
+    ∃ hx hy, "x" ↦ₖ hx ∗ "y" ↦ₖ hy ∗
+    (⌜hx = []⌝ ∨ (⌜hx = [(#1)]⌝ ∗ token γF1)) ∗
+    (⌜hy = []⌝ ∨ (⌜hy = [(#1)]⌝ ∗ token γF2)).
+
+  Lemma server_spec ip port :
+    ip = ip_of_address KVS_address →
+    port = port_of_address KVS_address →
+    SI_client_toolbox -∗
+    {{{ KVS_Init
+      ∗ KVS_address ⤳ (∅, ∅)
+      ∗ free_ports ip {[port]}
+      ∗ KVS_address ⤇ KVS_si }}}
+    server #KVS_address @[ip]
+    {{{ RET #(); True }}}.
+  Proof.
+    iIntros (Hip Hports) "(#Hinit_kvs & #Hinit_cli & #Hrd & #Hwr & #Hst & #Hcom) %Φ !> (? & ? & ? & ?) HΦ".
+    rewrite /server. wp_pures. rewrite Hip Hports.
+    by wp_apply ("Hinit_kvs" with "[$]").
+  Qed.
+
+  Lemma client_1_spec ip port γF1 γF2:
+  ip = ip_of_address client_1_addr →
+  port = port_of_address client_1_addr →
+  SI_client_toolbox -∗
+  {{{ inv client_inv_name (client_inv γF1 γF2)
+    ∗ token γF1
+    ∗ client_1_addr ⤳ (∅, ∅)
+    ∗ unallocated {[client_1_addr]}
+    ∗ KVS_ClientCanConnect client_1_addr
+    ∗ free_ports ip {[port]}
+    ∗ KVS_address ⤇ KVS_si }}}
+    transaction1_client $client_1_addr $KVS_address @[ip]
+  {{{ v, RET v; True }}}.
+  Proof.
+    iIntros (Hip Hports) "(#Hinit_kvs & #Hinit_cli & #Hrd & #Hwr & #Hst & #Hcom) %Φ !> (#Hinv & Htok & Hmsghis & Hunalloc
+    & Hports & Hcc & Hprot) HΦ".
+    rewrite /transaction1_client. wp_pures. rewrite Hip Hports.
+    wp_apply ("Hinit_cli" with "[$Hunalloc $Hprot $Hmsghis $Hports $Hcc]").
+    iIntros (rpc) "(Hcstate & #HiC)". wp_pures. rewrite /transaction1. wp_pures.
+    wp_apply ("Hst" $! rpc client_1_addr (⊤ ∖ ↑client_inv_name)); try solve_ndisj.
+    iInv (client_inv_name) as ">[%hx [%hy (Hkx & Hky & [->| (_ & Htok')] & Hhyp_y)]]" "Hclose";
+    try iDestruct (token_exclusive with "Htok Htok'") as "[]".
+    iModIntro. iFrame.
+    iExists {["x" := []; "y" := hy]}.
+    rewrite !big_sepM_insert; try set_solver.
+    rewrite big_sepM_empty.
+    iSplitL "Hkx Hky"; first iFrame.
+    iNext. iIntros "(Hcstate & (Hkx & Hky & _) & ((Hcx1 & Hcx2) & (Hcy1 & Hcy2 ) & _) & _)".
+    iMod ("Hclose" with "[Hkx Hky Hhyp_y]") as "_".
+    { iNext. iExists _, _. iFrame. by iLeft. }
+    iModIntro. wp_pures.
+    wp_apply ("Hrd" $! _ _ ⊤ with "[//][][$]"); first set_solver.
+    iModIntro.
+    iExists _.
+    iFrame.
+    iNext.
+    iIntros "Hcy1".
+    iModIntro.
+    wp_pures.
+    wp_apply ("Hwr" $! _ _  ⊤ _ (SerVal #1) with "[//][][$]"); first set_solver.
+    iModIntro.
+    iExists _, _.
+    iFrame.
+    iNext.
+    iIntros "(Hcx1 & Hcx2)".
+    iModIntro.
+    wp_pures.
+    wp_apply (commitT_spec rpc client_1_addr (⊤ ∖ ↑client_inv_name));
+    try solve_ndisj. iFrame "#".
+    iInv (client_inv_name) as ">[%hx' [%hy' (Hkx & Hky & [->| (_ & Htok')] & Hhyp_y)]]" "Hclose";
+    try iDestruct (token_exclusive with "Htok Htok'") as "[]".
+    iModIntro.
+    - iExists {["x" := []; "y" := hy']} , _, {["x" := (Some #1, true); "y" := (last hy, false)]}.
+      iFrame.
+      iSplitL "Hcx1 Hcx2 Hcy1 Hcy2 Hkx Hky".
+        + iSplitR. iPureIntro. set_solver.
+          iSplitR. iPureIntro. set_solver.
+          iSplitL "Hkx Hky".
+          rewrite !big_sepM_insert; try set_solver.
+          rewrite !big_sepM_empty. iFrame.
+          rewrite !big_sepM_insert; try set_solver.
+          rewrite !big_sepM_empty. iFrame.
+        + iNext. iIntros "[_ HBig]".
+          iMod ("Hclose" with "[Hhyp_y HBig Htok]") as "_".
+              * iNext. iExists _, _.
+                rewrite !(big_sepM2_insert); try set_solver.
+                iDestruct "HBig" as "((Hkx & _) & (Hky & _) & _)".
+                iFrame.
+                iSplitL "Htok".
+                iRight.
+                iFrame.
+                by iPureIntro.
+                iDestruct "Hhyp_y" as "[-> | (-> & Htoky)]".
+                iLeft.
+                iPureIntro.
+                destruct (last hy); done.
+                iRight.
+                iFrame.
+                iPureIntro.
+                destruct (last hy); done.
+              * iModIntro. by iApply "HΦ".
+  Qed.
+
+  Lemma client_2_spec ip port γF1 γF2:
+    ip = ip_of_address client_2_addr →
+    port = port_of_address client_2_addr →
+    SI_client_toolbox -∗
+    {{{ inv client_inv_name (client_inv γF1 γF2)
+      ∗ token γF2
+      ∗ client_2_addr ⤳ (∅, ∅)
+      ∗ unallocated {[client_2_addr]}
+      ∗ KVS_ClientCanConnect client_2_addr
+      ∗ free_ports ip {[port]}
+      ∗ KVS_address ⤇ KVS_si
+      ∗ GlobalInv }}}
+      transaction2_client $client_2_addr $KVS_address @[ip]
+    {{{ v, RET v; True }}}.
+  Proof.
+    iIntros (Hip Hports) "(#Hinit_kvs & #Hinit_cli & #Hrd & #Hwr & #Hst & #Hcom) %Φ !> (#Hinv & Htok & Hmsghis & Hunalloc
+    & Hports & Hcc & Hprot & #ginv) HΦ".
+    rewrite /transaction2_client. wp_pures. rewrite Hip Hports.
+    wp_apply ("Hinit_cli" with "[$Hunalloc $Hprot $Hmsghis $Hports $Hcc]").
+    iIntros (rpc) "(Hcstate & #HiC)". wp_pures. rewrite /transaction2. wp_pures.
+    wp_apply ("Hst" $! rpc client_2_addr (⊤ ∖ ↑client_inv_name)); try solve_ndisj.
+    iInv (client_inv_name) as ">[%hx [%hy (Hkx & Hky & Hhyp_x & [->| (_ & Htok')])]]" "Hclose";
+    try iDestruct (token_exclusive with "Htok Htok'") as "[]".
+    iModIntro. iFrame.
+    iExists {["x" := hx; "y" := []]}.
+    rewrite !big_sepM_insert; try set_solver.
+    rewrite big_sepM_empty.
+    iSplitL "Hkx Hky"; first iFrame.
+    iNext. iIntros "(Hcstate & (Hkx & Hky & _) & ((Hcx1 & Hcx2) & (Hcy1 & Hcy2 ) & _) & _)".
+    iMod ("Hclose" with "[Hkx Hky Hhyp_x]") as "_".
+    { iNext. iExists _, _. iFrame. by iLeft. }
+    iModIntro. wp_pures.
+    wp_apply ("Hrd" $! _ _ ⊤ with "[//][][$]"); first set_solver.
+    iModIntro.
+    iExists _.
+    iFrame.
+    iNext.
+    iIntros "Hcx1".
+    iModIntro.
+    wp_pures.
+    wp_apply ("Hwr" $! _ _  ⊤ _ (SerVal #1) with "[//][][$]"); first set_solver.
+    iModIntro.
+    iExists _, _.
+    iFrame.
+    iNext.
+    iIntros "(Hcy1 & Hcy2)".
+    iModIntro.
+    wp_pures.
+    wp_apply (commitT_spec rpc client_2_addr (⊤ ∖ ↑client_inv_name));
+    try solve_ndisj. iFrame "#".
+    iInv (client_inv_name) as ">[%hx' [%hy' (Hkx & Hky & Hhyp_x & [->| (_ & Htok')])]]" "Hclose";
+    try iDestruct (token_exclusive with "Htok Htok'") as "[]".
+    iModIntro.
+    - iExists {["x" := hx'; "y" := []]} , _, {["x" := (last hx, false); "y" := (Some #1, true)]}.
+      iFrame.
+      iSplitL "Hcx1 Hcx2 Hcy1 Hcy2 Hkx Hky".
+        + iSplitR. iPureIntro. set_solver.
+          iSplitR. iPureIntro. set_solver.
+          iSplitL "Hkx Hky".
+          rewrite !big_sepM_insert; try set_solver.
+          rewrite !big_sepM_empty. iFrame.
+          rewrite !big_sepM_insert; try set_solver.
+          rewrite !big_sepM_empty. iFrame.
+        + iNext. iIntros "[_ HBig]".
+          iMod ("Hclose" with "[Hhyp_x HBig Htok]") as "_".
+              * iNext. iExists _, _.
+                rewrite !(big_sepM2_insert); try set_solver.
+                iDestruct "HBig" as "((Hkx & _) & (Hky & _) & _)".
+                iFrame.
+                iSplitL "Hhyp_x".
+                iDestruct "Hhyp_x" as "[-> | (-> & Htokx)]".
+                iLeft.
+                iPureIntro.
+                destruct (last hx); done.
+                iRight.
+                iFrame.
+                iPureIntro.
+                destruct (last hx); done.
+                iRight.
+                iFrame.
+                by iPureIntro.
+              * iModIntro. by iApply "HΦ".
+  Qed.
+
+End proofs.
+
+Section proof_runner.
+
+Context `{!anerisG Mdl Σ, !SI_init, !KVSG Σ}.
+
+  Definition example_runner : expr :=
+    let: "serveraddr" := MakeAddress #"0.0.0.0" #80 in
+    let: "client1addr" := MakeAddress #"0.0.0.1" #80 in
+    let: "client2addr" := MakeAddress #"0.0.0.2" #80 in
+    Start "0.0.0.0" (server "serveraddr") ;;
+    Start "0.0.0.1" (transaction1_client "client1addr" "serveraddr") ;;
+    Start "0.0.0.2" (transaction2_client "client2addr" "serveraddr").
+
+  Lemma example_runner_spec :
+    {{{ server_addr ⤳ (∅, ∅)
+      ∗ client_1_addr ⤳ (∅, ∅)
+      ∗ client_2_addr ⤳ (∅, ∅)
+      ∗ unallocated {[server_addr]}
+      ∗ unallocated {[client_1_addr]}
+      ∗ unallocated {[client_2_addr]}
+      ∗ free_ip (ip_of_address server_addr)
+      ∗ free_ip (ip_of_address client_1_addr)
+      ∗ free_ip (ip_of_address client_2_addr) }}}
+      example_runner @["system"]
+    {{{ v, RET v; True }}}.
+  Proof.
+    iMod (SI_init_module _ {[client_1_addr; client_2_addr]})
+      as (SI_res) "(mem & KVS_Init & #Hginv & Hcc & #specs)";
+         first done.
+    iMod (own_alloc (Excl ())) as (γF1) "Hftk1"; first done.
+    iMod (own_alloc (Excl ())) as (γF2) "Hftk2"; first done.
+    iMod (inv_alloc client_inv_name ⊤ (client_inv γF1 γF2) with "[mem]") as "#Hinv".
+    { iNext. iExists [], [].
+    iDestruct (big_sepS_delete _ _ "x" with "mem") as "(Hx & mem)";
+    first set_solver.
+    iDestruct (big_sepS_delete _ _ "y" with "mem") as "(Hy & HKVSres)";
+    first set_solver. iFrame.
+    iSplitL; set_solver.
+    }
+    iIntros (Φ) "(Hsrvhist & Hcli1hist & Hcli2hist & Hsrvunalloc & Hcli1unalloc
+    & Hcli2unalloc & ? & ? & ?) HΦ".
+    rewrite /example_runner.
+    wp_pures.
+    wp_apply (aneris_wp_socket_interp_alloc_singleton KVS_si with "Hsrvunalloc").
+    iIntros "#HKVS_si".
+    wp_apply (aneris_wp_start {[80%positive]}).
+    iFrame.
+    iDestruct (big_sepS_delete _  _ client_1_addr with "Hcc")
+      as "(Hcc1 & Hcc)";
+    first set_solver.
+    iDestruct (big_sepS_delete _  _ client_2_addr with "Hcc")
+      as "(Hcc2 & Hcc)";
+    first set_solver.
+    iSplitR "Hsrvhist KVS_Init".
+    - iModIntro. wp_pures.
+      wp_apply (aneris_wp_start {[80%positive : port]}).
+      iFrame.
+      iSplitR "Hcli1hist Hcli1unalloc Hftk1 Hcc1".
+      + iModIntro. wp_pures.
+        wp_apply (aneris_wp_start {[80%positive : port]}).
+        iFrame.
+        iSplitR "Hcli2hist Hcli2unalloc Hftk2 Hcc2".
+        * by iApply "HΦ".
+        * iIntros "!> Hports". wp_apply (client_2_spec with "[$][$]"); done.
+      + iIntros "!> Hports". wp_apply (client_1_spec with "[$][$]"); done.
+    - iIntros "!> Hports". wp_apply (server_spec with "[$][$]"); done.
+  Qed.
+
+End proof_runner.
+
+Definition unit_model := model _ (λ _ _, False) ().
+Lemma unit_model_rel_finitary : aneris_model_rel_finitary unit_model.
+Proof. intros ?. apply finite_smaller_card_nat. apply _. Qed.
+
+Definition ips : gset string :=
+  {[ ip_of_address server_addr ; ip_of_address client_1_addr
+  ; ip_of_address client_2_addr ]}.
+
+Definition sa_dom : gset socket_address :=
+  {[ server_addr ; client_1_addr; client_2_addr ]}.
+
+Definition init_state :=
+  {|
+    state_heaps := {["system" := ∅ ]};
+    state_sockets := {["system" := ∅ ]};
+    state_ms := ∅;
+  |}.
+
+Theorem runner_safe :
+  aneris_adequate example_runner "system" init_state (λ _, True).
+Proof.
+  set (Σ := #[anerisΣ unit_model; KVSΣ]).
+  apply (@adequacy Σ unit_model _ _ ips sa_dom ∅ ∅ ∅);
+    [apply unit_model_rel_finitary| |set_solver..].
+  iIntros (dinvG). iIntros "!> Hunallocated Hhist Hfrag Hips Hlbl _ _ _ _".
+  iApply (example_runner_spec with "[Hunallocated Hhist Hfrag Hips Hlbl]" ).
+  2 : { iModIntro. done. }
+  do 2 (iDestruct (unallocated_split with "Hunallocated") as "[Hunallocated ?]";
+  [set_solver|]). iFrame.
+  do 2 (rewrite big_sepS_union; [|set_solver];
+  rewrite !big_sepS_singleton;
+  iDestruct "Hhist" as "[Hhist ?]"; iFrame).
+  do 2 (rewrite big_sepS_union; [|set_solver];
+  rewrite !big_sepS_singleton;
+  iDestruct "Hips" as "[Hips ?]"; iFrame).
+Qed.
